examples/ProcDec.v
@@ -1,7 +1,7 @@
 Require Import Bool String List.
 Require Import Lib.CommonTactics Lib.ilist Lib.Word Lib.Indexer Lib.StringBound.
 Require Import Lts.Syntax Lts.Notations Lts.Semantics Lts.Specialize Lts.Duplicate Lts.Equiv Lts.Tactics.
-Require Import Ex.SC Ex.Fifo Ex.MemAtomic.
+Require Import Ex.MemTypes Ex.SC Ex.Fifo Ex.MemAtomic.
 
 Set Implicit Arguments.
 
@@ -12,19 +12,22 @@ Set Implicit Arguments.
  *)
 Section ProcDec.
   Variable inName outName: string.
-  Variables addrSize valSize rfIdx: nat.
+  Variables addrSize lgDataBytes rfIdx: nat.
 
-  Variable dec: DecT 2 addrSize valSize rfIdx.
-  Variable execState: ExecStateT 2 addrSize valSize rfIdx.
-  Variable execNextPc: ExecNextPcT 2 addrSize valSize rfIdx.
+  Variable dec: DecT 2 addrSize lgDataBytes rfIdx.
+  Variable execState: ExecStateT 2 addrSize lgDataBytes rfIdx.
+  Variable execNextPc: ExecNextPcT 2 addrSize lgDataBytes rfIdx.
 
   Definition opLd : ConstT (Bit 2) := WO~0~0.
   Definition opSt : ConstT (Bit 2) := WO~0~1.
   Definition opHt : ConstT (Bit 2) := WO~1~0.
 
+  Definition RqFromProc := MemTypes.RqFromProc lgDataBytes (Bit addrSize).
+  Definition RsToProc := MemTypes.RsToProc lgDataBytes.
+
   (* Called method signatures *)
-  Definition memReq := MethodSig (inName .. "enq")(memAtomK addrSize valSize) : Void.
-  Definition memRep := MethodSig (outName .. "deq")() : memAtomK addrSize valSize.
+  Definition memReq := MethodSig (inName .. "enq")(RqFromProc) : Void.
+  Definition memRep := MethodSig (outName .. "deq")() : RsToProc.
   Definition halt := MethodSig "HALT"() : Void.
 
   Definition nextPc {ty} ppc st inst :=
@@ -38,9 +41,9 @@ Section ProcDec.
      Read st <- "rf";
      LET inst <- dec _ st ppc;
      Assert #inst@."opcode" == $$opLd;
-     Call memReq(STRUCT {  "type" ::= $$memLd;
-                           "addr" ::= #inst@."addr";
-                           "value" ::= $$Default });
+     Call memReq(STRUCT { "addr" ::= #inst@."addr";
+                          "op" ::= $$false;
+                          "data" ::= $$Default });
      Write "stall" <- $$true;
      Retv)%kami.
 
@@ -51,9 +54,9 @@ Section ProcDec.
      Read st <- "rf";
      LET inst <- dec _ st ppc;
      Assert #inst@."opcode" == $$opSt;
-     Call memReq(STRUCT {  "type" ::= $$opSt;
-                           "addr" ::= #inst@."addr";
-                           "value" ::= #inst@."value" });
+     Call memReq(STRUCT {  "addr" ::= #inst@."addr";
+                           "op" ::= $$true;
+                           "data" ::= #inst@."value" });
      Write "stall" <- $$true;
      Retv)%kami.
 
@@ -62,9 +65,8 @@ Section ProcDec.
      Read ppc <- "pc";
      Read st <- "rf";
      LET inst <- dec _ st ppc;
-     (* Assert #val@."type" == $$opLd; *)
      Assert #inst@."opcode" == $$opLd;
-     Write "rf" <- #st@[#inst@."reg" <- #val@."value"];
+     Write "rf" <- #st@[#inst@."reg" <- #val@."data"];
      Write "stall" <- $$false;
      nextPc ppc st inst)%kami.
 
@@ -73,7 +75,6 @@ Section ProcDec.
      Read ppc <- "pc";
      Read st <- "rf";
      LET inst <- dec _ st ppc;
-     (* Assert #val@."type" == $$opSt; *)
      Assert #inst@."opcode" == $$opSt;
      Write "stall" <- $$false;
      nextPc ppc st inst)%kami.
@@ -102,7 +103,7 @@ Section ProcDec.
 
   Definition procDec := MODULE {
     Register "pc" : Bit addrSize <- Default
-    with Register "rf" : Vector (Bit valSize) rfIdx <- Default
+    with Register "rf" : Vector (Data lgDataBytes) rfIdx <- Default
     with Register "stall" : Bool <- false
 
     with Rule "reqLd" := reqLd
@@ -116,36 +117,33 @@ Section ProcDec.
 End ProcDec.
 
 Hint Unfold procDec : ModuleDefs.
-Hint Unfold opLd opSt opHt
+Hint Unfold RqFromProc RsToProc opLd opSt opHt
      memReq memRep halt nextPc
      reqLd reqSt repLd repSt execHt execNm : MethDefs.
 
 Section ProcDecM.
-  Variables addrSize fifoSize valSize rfIdx: nat.
+  Variables addrSize fifoSize lgDataBytes rfIdx: nat.
 
-  Variable dec: DecT 2 addrSize valSize rfIdx.
-  Variable execState: ExecStateT 2 addrSize valSize rfIdx.
-  Variable execNextPc: ExecNextPcT 2 addrSize valSize rfIdx.
+  Variable dec: DecT 2 addrSize lgDataBytes rfIdx.
+  Variable execState: ExecStateT 2 addrSize lgDataBytes rfIdx.
+  Variable execNextPc: ExecNextPcT 2 addrSize lgDataBytes rfIdx.
 
   Definition pdec := procDec "Ins"%string "Outs"%string dec execState execNextPc.
 
-  Definition pdecf := ConcatMod pdec (iom addrSize fifoSize (Bit valSize)).
+  Definition pdecf := ConcatMod pdec (iom addrSize fifoSize lgDataBytes).
   Definition pdecfs (i: nat) := duplicate pdecf i.
-  Definition procDecM (n: nat) := ConcatMod (pdecfs n) (minst addrSize (Bit valSize) n).
+  Definition procDecM (n: nat) := ConcatMod (pdecfs n) (minst addrSize lgDataBytes n).
 
 End ProcDecM.
 
 Hint Unfold pdec pdecf pdecfs procDecM : ModuleDefs.
 
 Section Facts.
-  Variables addrSize fifoSize valSize rfIdx: nat.
+  Variables addrSize fifoSize lgDataBytes rfIdx: nat.
 
-  Variable dec: DecT 2 addrSize valSize rfIdx.
-  Variable execState: ExecStateT 2 addrSize valSize rfIdx.
-  Variable execNextPc: ExecNextPcT 2 addrSize valSize rfIdx.
-  (* Hypotheses (HdecEquiv: DecEquiv dec) *)
-  (*            (HexecEquiv_1: ExecEquiv_1 dec exec) *)
-  (*            (HexecEquiv_2: ExecEquiv_2 dec exec). *)
+  Variable dec: DecT 2 addrSize lgDataBytes rfIdx.
+  Variable execState: ExecStateT 2 addrSize lgDataBytes rfIdx.
+  Variable execNextPc: ExecNextPcT 2 addrSize lgDataBytes rfIdx.
 
   Lemma pdecf_ModEquiv:
     forall fsz m,
