examples/ProcDecSCN.v
@@ -9,14 +9,11 @@ Require Import Ex.ProcDec Ex.ProcDecInl Ex.ProcDecInv Ex.ProcDecSC.
 Set Implicit Arguments.
 
 Section ProcDecSCN.
-  Variables addrSize fifoSize valSize rfIdx: nat.
+  Variables addrSize fifoSize lgDataBytes rfIdx: nat.
 
-  Variable dec: DecT 2 addrSize valSize rfIdx.
-  Variable execState: ExecStateT 2 addrSize valSize rfIdx.
-  Variable execNextPc: ExecNextPcT 2 addrSize valSize rfIdx.
-  (* Hypotheses (HdecEquiv: DecEquiv dec) *)
-  (*            (HexecEquiv_1: ExecEquiv_1 dec exec) *)
-  (*            (HexecEquiv_2: ExecEquiv_2 dec exec). *)
+  Variable dec: DecT 2 addrSize lgDataBytes rfIdx.
+  Variable execState: ExecStateT 2 addrSize lgDataBytes rfIdx.
+  Variable execNextPc: ExecNextPcT 2 addrSize lgDataBytes rfIdx.
 
   Variable n: nat.
   
